Splinter/CoordinationLayer/CoordProgramRefinement.i.dfy
@@ -1,0 +1,81 @@
+include "../IOSystem.s.dfy"
+include "../ProofObligations.s.dfy"
+include "CoordProgramMod.i.dfy"
+
+// This module shows refinement of CoordProgram to CrashTolerantMapSpecMod,
+// thereby functioning as the top layer in a refinement stack for program
+// models in refinement layers below.
+module CoordProgramRefinement {
+  import opened CoordProgramMod
+  import MapSpecMod
+
+  function I(v: CoordProgramMod.Variables) : CrashTolerantMapSpecMod.Variables
+  {
+    if !Inv(v)
+    then CrashTolerantMapSpecMod.InitState()
+    else if v.phase.SuperblockUnknown?
+      then v.stableSuperblock.journal.AsCrashTolerantMapSpec(v.stableSuperblock.mapadt)
+      else v.journal.AsCrashTolerantMapSpec(v.mapadt)
+    
+  }
+
+  predicate Inv(v: CoordProgramMod.Variables)
+  {
+    && v.WF()
+    && v.stableSuperblock.mapadt.seqEnd == v.stableSuperblock.journal.msgSeq.seqStart
+    && (!v.phase.SuperblockUnknown? ==>
+      && v.mapadt.seqEnd == v.journal.msgSeq.seqStart
+    )
+  }
+
+  lemma InitRefines(v: CoordProgramMod.Variables)
+    requires CoordProgramMod.Init(v)
+    ensures Inv(v)
+    ensures I(v) == CrashTolerantMapSpecMod.InitState()
+  {
+    assert JournalInterpTypeMod.Mkfs().SyncReqsAt(0) == {}; // trigger set comprehension
+  }
+
+  lemma InvInductive(v: CoordProgramMod.Variables, v': CoordProgramMod.Variables, uiop: CoordProgramMod.UIOp)
+    requires Inv(v)
+    requires CoordProgramMod.Next(v, v', uiop)
+    ensures Inv(v')
+  {
+    var step :| NextStep(v, v', uiop, step);
+    match step {
+      case RecoverStep(puts) => {
+        assert Inv(v'); // here
+      }
+      case QueryStep(key, val) => {
+        assert Inv(v');
+      }
+      case PutStep() => {
+        assert Inv(v'); // here
+      }
+//    case JournalInternalStep(sk) => { assert Inv(v'); }
+//    case SplinterTreeInternalStep(sk) => { assert Inv(v'); }
+      case ReqSyncStep(syncReqId) => {
+        assert Inv(v');
+      }
+      case CompleteSyncStep(syncReqId) => {
+        assert Inv(v');
+      }
+      case CommitStartStep(seqBoundary) => {
+        assert Inv(v');
+      }
+      case CommitCompleteStep() => {
+        assert Inv(v'); // here
+      }
+    }
+  }
+
+  lemma NextRefines(v: CoordProgramMod.Variables, v': CoordProgramMod.Variables, uiop: CoordProgramMod.UIOp)
+    requires Inv(v)
+    requires CoordProgramMod.Next(v, v', uiop)
+    ensures Inv(v')
+    ensures CrashTolerantMapSpecMod.Next(I(v), I(v'), uiop)
+  {
+    InvInductive(v, v', uiop);
+    assert CrashTolerantMapSpecMod.Next(I(v), I(v'), uiop);
+  }
+}
